src/LocalReasoning.v
@@ -49,7 +49,7 @@ Proof.
   assert (σ' ⊨ (Singleton Loc v) : hot).
   + eapply local_reasoning;
       eauto using stk_theorem with pM stk wf lia.
-    eapply scopability_theorem in H; eauto with pM wf lia; steps.
+    eapply scp_theorem in H; eauto with pM wf lia; steps.
   + eapply H3; eauto using In_singleton.
 Qed.
 
